Working abstraction layer with types and correction on compilation function. Elimination of dead guard in forever loop.

Interface.v
@@ -1,4 +1,5 @@
 Require Import lib.Integers.
+Require Import lib.Floats.
 Require Import Rustre.Common.
 Require Import common.Smallstep.
 Require Import common.Events.
@@ -8,44 +9,188 @@ Require Import Rustre.Minimp.Syntax.
 Require Import Rustre.Minimp.Semantics.
 
 (* Interface avec CompCert *)
-Inductive val'' : Type :=
-| Vundef : val''
-| Vint : Int.int -> val''.
+Inductive val'': Type :=
+(* | Vundef: val'' *)
+| Vint: Int.int -> val''
+| Vfloat: float32 -> val''.
 
-Inductive unary_op' : Type :=
-| Opposite : unary_op'
-| Negation : unary_op'.
+Inductive typ': Type :=
+| Tbool
+| Tvoid
+| Tint
+| Tfloat.
 
-Inductive binary_op' : Type :=
-| Add : binary_op'
-| Sub : binary_op'
-| Mul : binary_op'.
+Inductive unary_op': Type :=
+| Opposite
+| Negation.
+
+Inductive binary_op': Type :=
+| Add
+| Sub
+| Mul.
 
 Definition zero := Int.zero.
 Definition one := Int.one.
-Definition Vzero := Vint Int.zero.
 
-Module Op <: OPERATORS.
-  Definition val' := val''.
+Module Export Op <: OPERATORS.
+  Definition val': Type := val''.
               
   Inductive val: Type :=
   | Vbool: bool -> val
   | Val: val' -> val.
 
-  Definition typ := nat.
-  
+  Definition Vzero := Val (Vint Int.zero).
+
+  Definition typ := typ'.
+
+  Definition typ_of_val (v: val): typ :=
+    match v with
+    | Vbool _ => Tbool
+    | Val v =>
+      match v with
+      (* | Vundef => Tvoid *)
+      | Vint _ => Tint
+      | Vfloat _ => Tfloat
+      end
+    end.
+    
   Definition unary_op := unary_op'.
   Definition binary_op := binary_op'.
 
-  Definition of_bool (b: bool) := Vint (if b then one else zero).
+  Definition opt (v: val'): option val := Some (Val v).
+  
+  Definition of_bool (b: bool): val' := Vint (if b then one else zero).
 
-  Definition sem_val_unary (sem: val' -> option val) (v: val) :=
+  Definition sem_val_unary (sem: val' -> typ -> option val) (v: val): typ -> option val :=
     match v with
     | Vbool b => sem (of_bool b)   
     | Val v => sem v
     end.
+  
+  Definition sem_opposite: val -> typ -> option val :=
+    let sem v ty :=
+        match v, ty with
+        | Vint n, (Tint | Tbool) => opt (Vint (Int.neg n))
+        | Vfloat f, Tfloat => opt (Vfloat (Float32.neg f))
+        | _, _ => None
+        end
+    in sem_val_unary sem.
+  
+  Definition sem_negation: val -> typ -> option val :=
+    let sem v ty :=
+        match v, ty with
+        | Vint n, (Tint | Tbool) => opt (of_bool (Int.eq n zero))
+        | Vfloat f, Tfloat => opt (of_bool (Float32.cmp Ceq f Float32.zero))
+        | _, _ => None
+        end
+    in sem_val_unary sem.
+    
+  Definition sem_unary (op: unary_op): val -> typ -> option val :=
+    match op with
+    | Opposite => sem_opposite 
+    | Negation => sem_negation 
+    end.
 
-  Definition sem_val_binary (sem: val' -> val' -> option val) (v1 v2: val) :=
+  Inductive classify_cast_cases :=
+  | cast_case_neutral
+  | cast_case_f2bool
+  | cast_case_i2bool
+  | cast_case_f2i
+  | cast_case_f2f
+  | cast_case_i2f
+  | cast_case_void
+  | cast_case_default.
+  
+  Definition classify_cast (tfrom tto: typ) : classify_cast_cases :=
+    match tto, tfrom with
+    | Tint, (Tint | Tbool) => cast_case_neutral
+    | Tbool, Tfloat => cast_case_f2bool
+    | Tbool, Tint => cast_case_i2bool
+    | Tint, Tfloat => cast_case_f2i
+    | Tfloat, Tfloat => cast_case_f2f
+    | Tfloat, (Tint | Tbool) => cast_case_i2f 
+    | Tvoid, _ => cast_case_void
+    | _, _ => cast_case_default
+    end.
+
+  Definition sem_cast (v: val') (ty1 ty2: typ) : option val' :=
+    match classify_cast ty1 ty2 with
+    | cast_case_neutral =>
+      match v with
+      | Vint _ => Some v
+      | _ => None
+      end
+    | cast_case_f2bool =>
+      match v with
+      | Vfloat f => Some (of_bool (Float32.cmp Ceq f Float32.zero))
+      | _ => None
+      end
+    | cast_case_i2bool =>
+      match v with
+      | Vint i => Some (of_bool (Int.eq i Int.zero))
+      | _ => None
+      end
+    | cast_case_f2i =>
+      match v with
+      | Vfloat f =>
+        match Float32.to_int f with
+        | Some i => Some (Vint i)
+        | None => None
+        end
+      | _ => None
+      end
+    | cast_case_f2f =>
+      match v with
+      | Vfloat f => Some (Vfloat f)
+      | _ => None
+      end
+    | cast_case_i2f =>
+      match v with
+      | Vint i => Some (Vfloat (Float32.of_int i))
+      | _ => None
+      end
+    | cast_case_void => Some v
+    | cast_case_default => None
+    end.
+
+  Definition binarith_type (ty1 ty2: typ) : typ :=
+    match ty1, ty2 with
+    | (Tint | Tbool), (Tint | Tbool) => Tint
+    | Tfloat, Tfloat
+    | (Tint | Tbool), Tfloat
+    | Tfloat, (Tint | Tbool) => Tfloat
+    | _, _ => Tvoid
+    end.
+
+  Definition sem_binarith
+    (sem_int: int -> int -> option val)
+    (sem_float: float32 -> float32 -> option val)
+    (v1 v2: val') (ty1 ty2: typ): option val :=
+    let ty := binarith_type ty1 ty2 in
+    match sem_cast v1 ty1 ty with
+    | None => None
+    | Some v1' =>
+      match sem_cast v2 ty2 ty with
+      | None => None
+      | Some v2' =>
+        match ty with
+        | Tint =>
+          match v1', v2' with
+          | Vint n1, Vint n2 => sem_int n1 n2
+          | _, _ => None
+          end
+        | Tfloat =>
+          match v1', v2' with
+          | Vfloat f1, Vfloat f2 => sem_float f1 f2
+          | _, _ => None
+          end
+        | bin_default => None
+        end
+      end
+    end.
+  
+  Definition sem_val_binary (sem: val' -> val' -> typ -> typ -> option val) (v1 v2: val)
+    : typ -> typ -> option val :=
     match v1, v2 with
     | Vbool b1, Vbool b2 => sem (of_bool b1) (of_bool b2)
     | Val v1, Vbool b2 => sem v1 (of_bool b2)
@@ -53,109 +198,116 @@ Module Op <: OPERATORS.
     | Val v1, Val v2 => sem v1 v2
     end.
   
-  Definition sem_opposite: val -> option val :=
-    let sem v :=
-        match v with
-        | Vundef => None
-        | Vint n => Some (Val (Vint (Int.neg n)))
-        end
-    in sem_val_unary sem.
+  Definition sem_add: val -> val -> typ -> typ -> option val :=
+    let sem_int n1 n2 := opt (Vint (Int.add n1 n2)) in
+    let sem_float f1 f2 := opt (Vfloat (Float32.add f1 f2)) in
+    sem_val_binary (sem_binarith sem_int sem_float).
+
+  Definition sem_sub: val -> val -> typ -> typ -> option val :=
+    let sem_int n1 n2 := opt (Vint (Int.sub n1 n2)) in
+    let sem_float f1 f2 := opt (Vfloat (Float32.sub f1 f2)) in
+    sem_val_binary (sem_binarith sem_int sem_float).
+
+  Definition sem_mul: val -> val -> typ -> typ -> option val :=
+    let sem_int n1 n2 := opt (Vint (Int.mul n1 n2)) in
+    let sem_float f1 f2 := opt (Vfloat (Float32.mul f1 f2)) in
+    sem_val_binary (sem_binarith sem_int sem_float).
   
-  Definition sem_negation: val -> option val :=
-    let sem v :=
-        match v with
-        | Vundef => None
-        | Vint n => Some (Val (Vint (if (Int.eq n zero) then one else zero)))
-        end
-    in sem_val_unary sem.
+  Definition sem_binary (op: binary_op) (v1: val) (ty1: typ) (v2: val) (ty2: typ): option val :=
+    (match op with
+    | Add => sem_add
+    | Sub => sem_sub
+    | Mul => sem_mul
+    end) v1 v2 ty1 ty2.
     
-  Definition sem_unary (op : unary_op): val -> option val :=
-    match op with
-    | Opposite => sem_opposite 
-    | Negation => sem_negation 
-    end.
+  (* Lemma val_dec: forall v1 v2: val, {v1 = v2} + {v1 <> v2}. *)
+  (* Proof. *)
+  (*   decide equality. *)
+  (*   apply Bool.bool_dec. *)
+  (*   decide equality. *)
+  (*   apply Int.eq_dec. *)
+  (*   apply Float.eq_dec. *)
+  (* Qed. *)
 
-  Definition sem_plus: val -> val -> option val :=
-    let sem v1 v2 :=
-        match v1, v2 with
-        | Vint n1, Vint n2 => Some (Val (Vint (Int.add n1 n2)))
-        | _, _ => None
-        end
-    in sem_val_binary sem.
-
-  Definition sem_minus: val -> val -> option val :=
-    let sem v1 v2 :=
-        match v1, v2 with
-        | Vint n1, Vint n2 => Some (Val (Vint (Int.sub n1 n2)))
-        | _, _ => None
-        end
-    in sem_val_binary sem.
-
-  Definition sem_mult: val -> val -> option val :=
-    let sem v1 v2 :=
-        match v1, v2 with
-        | Vint n1, Vint n2 => Some (Val (Vint (Int.mul n1 n2)))
-        | _, _ => None
-        end
-    in sem_val_binary sem.
-  
-  Definition sem_binary (op : binary_op): val -> val -> option val :=
-    match op with
-    | Add => sem_plus
-    | Sub => sem_minus
-    | Mul => sem_mult
-    end.
-    
-  Lemma val_dec : forall v1 v2 : val, {v1 = v2} + {v1 <> v2}.
-  Proof. decide equality; [apply Bool.bool_dec | decide equality; apply Int.eq_dec]. Qed.
-  Definition val_eqb (v1 v2 : val) : bool :=
+  Definition val_eqb (v1 v2: val): bool :=
     match v1, v2 with
     | Vbool b1, Vbool b2 => Bool.eqb b1 b2
     | Val v1, Val v2 =>
       match v1, v2 with
-      | Vundef, Vundef => true
+      (* | Vundef, Vundef => true *)
       | Vint n1, Vint n2 => Int.eq n1 n2
+      | Vfloat f1, Vfloat f2 => if Float32.eq_dec f1 f2 then true else false
       | _, _ => false
       end
     | _, _ => false
     end.
 
-  Lemma unop_dec : forall op1 op2 : unary_op, {op1 = op2} + {op1 <> op2}.
-  Proof. decide equality. Qed.
-  Definition unop_eqb (op1 op2 : unary_op) := if unop_dec op1 op2 then true else false.
-
-  Lemma binop_dec : forall op1 op2 : binary_op, {op1 = op2} + {op1 <> op2}.
-  Proof. decide equality. Qed.
-  Definition binop_eqb (op1 op2 : binary_op) := if binop_dec op1 op2 then true else false.
+  Definition typ_eqb (ty1 ty2: typ): bool :=
+    match ty1, ty2 with
+    | Tbool, Tbool
+    | Tvoid, Tvoid
+    | Tint, Tint
+    | Tfloat, Tfloat => true
+    | _, _ => false
+    end.
   
-  Theorem val_eqb_true_iff : forall v1 v2, val_eqb v1 v2 = true <-> v1 = v2.
+  Lemma unop_dec: forall op1 op2: unary_op, {op1 = op2} + {op1 <> op2}.
+  Proof. decide equality. Qed.
+  Definition unop_eqb (op1 op2: unary_op) := if unop_dec op1 op2 then true else false.
+
+  Lemma binop_dec: forall op1 op2: binary_op, {op1 = op2} + {op1 <> op2}.
+  Proof. decide equality. Qed.
+  Definition binop_eqb (op1 op2: binary_op) := if binop_dec op1 op2 then true else false.
+  
+  Theorem val_eqb_true_iff: forall v1 v2, val_eqb v1 v2 = true <-> v1 = v2.
   Proof.
     intros v1 v2; unfold val_eqb; destruct v1 as [b1|v1], v2 as [b2|v2];
-    try destruct b1, b2; try destruct v1 as [|n1], v2 as [|n2]; try intuition discriminate.
-    split; intro H.
-    - pose proof (Int.eq_spec n1 n2) as Heq; rewrite H in Heq; now do 2 f_equal.
-    - inversion H; apply Int.eq_true.
+    try destruct b1, b2; try destruct v1 as [n1|f1], v2 as [n2|f2];
+    try intuition discriminate.
+    - split; intro H.
+      + pose proof (Int.eq_spec n1 n2) as Heq; rewrite H in Heq; now do 2 f_equal.
+      + inversion H; apply Int.eq_true.
+    - split; intro H.
+      + destruct (Float32.eq_dec f1 f2).
+        * now inversion e.
+        * discriminate.
+      + destruct (Float32.eq_dec f1 f2); auto.
+        exfalso; apply n; now inversion H.
   Qed.
 
-  Theorem val_eqb_false_iff : forall v1 v2, val_eqb v1 v2 = false <-> v1 <> v2.
+  Theorem val_eqb_false_iff: forall v1 v2, val_eqb v1 v2 = false <-> v1 <> v2.
   Proof.
     intros v1 v2; unfold val_eqb; destruct v1 as [b1|v1], v2 as [b2|v2];
-    try destruct b1, b2; try destruct v1 as [|n1], v2 as [|n2]; try intuition discriminate.
-    split; intros H.
-    - intro Hf; pose proof (Int.eq_spec n1 n2) as Hneq; rewrite H in Hneq; inversion Hf as [Heq]; contradiction. 
-    - apply Int.eq_false; intro Heq; apply H; now do 2 f_equal.
+    try destruct b1, b2; try destruct v1 as [n1|f1], v2 as [n2|f2];
+    try intuition discriminate.
+    - split; intros H.
+      + intro Hf; pose proof (Int.eq_spec n1 n2) as Hneq; rewrite H in Hneq;
+        inversion Hf as [Heq]; contradiction. 
+      + apply Int.eq_false; intro Heq; apply H; now do 2 f_equal.
+    - split; intro H.
+      + destruct (Float32.eq_dec f1 f2).
+        * discriminate.
+        * intro H'; apply n; now inversion H'.
+      + destruct (Float32.eq_dec f1 f2); auto.
+        exfalso; apply H; now inversion e.
   Qed.
 
-  Theorem unop_eqb_true_iff : forall op1 op2, unop_eqb op1 op2 = true <-> op1 = op2.
+  Theorem typ_eqb_true_iff : forall t1 t2, typ_eqb t1 t2 = true <-> t1 = t2.
+  Proof. intros ty1 ty2; destruct ty1, ty2; intuition discriminate. Qed.
+  
+  Theorem typ_eqb_false_iff : forall t1 t2, typ_eqb t1 t2 = false <-> t1 <> t2.
+  Proof. intros ty1 ty2; destruct ty1, ty2; intuition discriminate. Qed.
+
+  Theorem unop_eqb_true_iff: forall op1 op2, unop_eqb op1 op2 = true <-> op1 = op2.
   Proof. intros op1 op2; unfold unop_eqb; destruct (unop_dec op1 op2); intuition discriminate. Qed.
   
-  Theorem unop_eqb_false_iff : forall op1 op2, unop_eqb op1 op2 = false <-> op1 <> op2.
+  Theorem unop_eqb_false_iff: forall op1 op2, unop_eqb op1 op2 = false <-> op1 <> op2.
   Proof. intros op1 op2; unfold unop_eqb; destruct (unop_dec op1 op2); intuition. Qed.
 
-  Theorem binop_eqb_true_iff : forall op1 op2, binop_eqb op1 op2 = true <-> op1 = op2. 
+  Theorem binop_eqb_true_iff: forall op1 op2, binop_eqb op1 op2 = true <-> op1 = op2. 
   Proof. intros op1 op2; unfold binop_eqb; destruct (binop_dec op1 op2); intuition discriminate. Qed.
   
-  Theorem binop_eqb_false_iff : forall op1 op2, binop_eqb op1 op2 = false <-> op1 <> op2. 
+  Theorem binop_eqb_false_iff: forall op1 op2, binop_eqb op1 op2 = false <-> op1 <> op2. 
   Proof. intros op1 op2; unfold binop_eqb; destruct (binop_dec op1 op2); intuition. Qed.
 
 End Op.
@@ -182,7 +334,7 @@ Inductive step: genv -> state -> trace -> state -> Prop :=
     step ge (State H S Skip) t StopState.
 
 Parameter convert_mem: mem -> heap * stack.
-Inductive initial_state (ge : genv) (p: program): state -> Prop :=
+Inductive initial_state (ge: genv) (p: program): state -> Prop :=
   IniState: forall b f m0 H0 S0,
     let p' := convert_prog p in
     Genv.init_mem p' = Some m0 ->
